Improve program simulation definition: now future program should satisfy a weaker notion of simulation.

backend/RTLSim.v
@@ -24,52 +24,52 @@ Definition state_mem (st:state): mem :=
 
 Section LSIM.
 
-Variable (Mrel:Type).
-Variable (Mrel_ops:MREL_ops Mrel).
+Variable (mrelT:Type).
+Variable (mrelT_ops:mrelT_opsT mrelT).
 
-Section LSIM_FUNC.
+Section FUNCTION_LSIM.
 
 Variable (ge_src ge_tgt:genv).
 
-Section LSIM_STATE.
+Section STATE_LSIM.
 
 Variable (cs_entry_src cs_entry_tgt:list stackframe).
-Variable (mrel_entry:Mrel).
+Variable (mrel_entry:mrelT).
 
-Inductive _lsim_state
-          (lsim_state: Mrel -> WF.t -> state -> state -> Prop)
-          (mrel:Mrel) (i:WF.t) (st_src st_tgt:state): Prop :=
-| _lsim_state_error
+Inductive _state_lsim
+          (state_lsim: mrelT -> WF.t -> state -> state -> Prop)
+          (mrel:mrelT) (i:WF.t) (st_src st_tgt:state): Prop :=
+| _state_lsim_error
     st2_src (Hst_src: star step ge_src st_src E0 st2_src)
     (Hnostep: nostep step ge_src st2_src)
-| _lsim_state_return
+| _state_lsim_return
     st2_src (Hst_src: star step ge_src st_src E0 st2_src)
     val2_src mem2_src (Hst2_src: st2_src = Returnstate cs_entry_src val2_src mem2_src)
     val_tgt mem_tgt (Hst_tgt: st_tgt = Returnstate cs_entry_tgt val_tgt mem_tgt)
-    (mrel2:Mrel) (Hmrel2: Mrel_ops.(sem) mrel2 mem2_src mem_tgt)
-    (Hmrel2_le: Mrel_ops.(le) mrel mrel2)
-    (Hmrel2_le_public: Mrel_ops.(le_public) mrel_entry mrel2)
-| _lsim_state_call
+    (mrel2:mrelT) (Hmrel2: mrelT_ops.(sem) mrel2 mem2_src mem_tgt)
+    (Hmrel2_le: mrelT_ops.(le) mrel mrel2)
+    (Hmrel2_le_public: mrelT_ops.(le_public) mrel_entry mrel2)
+| _state_lsim_call
     st2_src (Hst_src: star step ge_src st_src E0 st2_src)
     res2_src fundef2_src sp2_src pc2_src rs2_src stack2_src fundef3_src args2_src mem2_src
     (Hst2_src: st2_src = Callstate ((Stackframe res2_src fundef2_src sp2_src pc2_src rs2_src)::stack2_src) fundef3_src args2_src mem2_src)
     res2_tgt fundef2_tgt sp2_tgt pc2_tgt rs2_tgt stack2_tgt fundef3_tgt args2_tgt mem2_tgt
     (Hst_tgt: st_tgt = Callstate ((Stackframe res2_tgt fundef2_tgt sp2_tgt pc2_tgt rs2_tgt)::stack2_tgt) fundef3_tgt args2_tgt mem2_tgt)
-    (Hfundef2: True) (* TODO: fundef2_src and fundef_tgt shall be equivalent *)
-    (Hargs: True) (* TODO: args2_src and args_tgt shall be equivalent *)
-    (mrel2:Mrel) (Hmrel2: Mrel_ops.(sem) mrel2 mem2_src mem2_tgt)
-    (Hmrel2_le: Mrel_ops.(le) mrel mrel2)
+    (Hfundef2: exists b, ge_src.(Genv.genv_funs) ! b = Some fundef3_src /\ ge_tgt.(Genv.genv_funs) ! b = Some fundef3_tgt)
+    (Hargs: list_forall2 (mrelT_ops.(sem_value) mrel) args2_src args2_tgt)
+    (mrel2:mrelT) (Hmrel2: mrelT_ops.(sem) mrel2 mem2_src mem2_tgt)
+    (Hmrel2_le: mrelT_ops.(le) mrel mrel2)
     (Hreturn:
        forall mrel3 st3_src st3_tgt mem3_src mem3_tgt vres_src vres_tgt
-              (Hvres: True) (* TODO: vres shall be equivalent *)
+              (Hvres: mrelT_ops.(sem_value) mrel3 vres_src vres_tgt)
               (Hst3_src: st3_src = State stack2_src fundef2_src sp2_src pc2_src (rs2_src#res2_src <- vres_src) mem3_src)
               (Hst3_tgt: st3_tgt = State stack2_tgt fundef2_tgt sp2_tgt pc2_tgt (rs2_tgt#res2_tgt <- vres_tgt) mem3_tgt)
-              (Hmrel3_le: Mrel_ops.(le_public) mrel2 mrel3)
-              (Hst3_mem: Mrel_ops.(sem) mrel3 mem3_src mem3_tgt),
+              (Hmrel3_le: mrelT_ops.(le_public) mrel2 mrel3)
+              (Hst3_mem: mrelT_ops.(sem) mrel3 mem3_src mem3_tgt),
        exists i3,
-         lsim_state mrel3 i3 st3_src st3_tgt)
+         state_lsim mrel3 i3 st3_src st3_tgt)
 
-| _lsim_state_step
+| _state_lsim_step
     (Hprogress: exists evt st2_tgt, step ge_tgt st_tgt evt st2_tgt)
     (Hpreserve:
        forall evt st3_tgt (Hst3_tgt: step ge_tgt st_tgt evt st3_tgt),
@@ -77,30 +77,30 @@ Inductive _lsim_state
          star step ge_src st_src E0 st2_src /\
        exists i3 st3_src,
          indexed_step step ge_src (Indexed.mk i st2_src) evt (Indexed.mk i3 st3_src) /\
-       exists (mrel3:Mrel),
-         Mrel_ops.(le) mrel mrel3 /\
-         Mrel_ops.(sem) mrel3 (state_mem st3_src) (state_mem st3_tgt) /\
-         lsim_state mrel3 i3 st3_src st3_tgt)
+       exists (mrel3:mrelT),
+         mrelT_ops.(le) mrel mrel3 /\
+         mrelT_ops.(sem) mrel3 (state_mem st3_src) (state_mem st3_tgt) /\
+         state_lsim mrel3 i3 st3_src st3_tgt)
 .
-Hint Constructors _lsim_state.
+Hint Constructors _state_lsim.
 
-Lemma lsim_state_mon: monotone4 _lsim_state.
+Lemma state_lsim_mon: monotone4 _state_lsim.
 Proof.
   repeat intro; destruct IN; eauto.
-  - eapply _lsim_state_call; eauto.
+  - eapply _state_lsim_call; eauto.
     intros. exploit Hreturn; eauto.
     intros [i3 Hsim]. exists i3. auto.
-  - eapply _lsim_state_step; eauto.
+  - eapply _state_lsim_step; eauto.
     intros. exploit Hpreserve; eauto.
     intros [st2_src [Hst2_src [i3 [st3_src [Hst3_src [mrel3 [Hmrel3_le [Hmrel3 Hr]]]]]]]].
     eexists. split; eauto.
     eexists. eexists. split; eauto.
 Qed.
 
-Definition lsim_state: _ -> _ -> _ -> _ -> Prop :=
-  paco4 _lsim_state bot4.
+Definition state_lsim: _ -> _ -> _ -> _ -> Prop :=
+  paco4 _state_lsim bot4.
 
-End LSIM_STATE.
+End STATE_LSIM.
 
 Definition lsim_func_aux
            mrel_init func_src func_tgt: Prop :=
@@ -109,9 +109,9 @@ Definition lsim_func_aux
     cs_entry_src cs_entry_tgt
     args_src args_tgt
     mem2_src mem2_tgt stk_src stk_tgt rs_src rs_tgt st_src st_tgt
-    (Hmrel_entry_le: Mrel_ops.(le) mrel_init mrel_entry)
-    (Hmrel_entry: Mrel_ops.(sem) mrel_entry mem_entry_src mem_entry_tgt)
-    (Hargs: True) (* TODO: args_src and args_tgt shall be equivalent *)
+    (Hmrel_entry_le: mrelT_ops.(le) mrel_init mrel_entry)
+    (Hmrel_entry: mrelT_ops.(sem) mrel_entry mem_entry_src mem_entry_tgt)
+    (Hargs: list_forall2 (mrelT_ops.(sem_value) mrel_entry) args_src args_tgt)
     (Hstk_src: Mem.alloc mem_entry_src 0 func_src.(fn_stacksize) = (mem2_src, stk_src))
     (Hstk_tgt: Mem.alloc mem_entry_tgt 0 func_tgt.(fn_stacksize) = (mem2_tgt, stk_tgt))
     (Hrs_src: rs_src = init_regs args_src func_src.(fn_params))
@@ -119,36 +119,36 @@ Definition lsim_func_aux
     (Hst_src: st_src = State cs_entry_src func_src (Vptr stk_src Int.zero) func_src.(fn_entrypoint) rs_src mem2_src)
     (Hst_tgt: st_tgt = State cs_entry_tgt func_tgt (Vptr stk_tgt Int.zero) func_tgt.(fn_entrypoint) rs_tgt mem2_tgt),
   exists i,
-    lsim_state
+    state_lsim
       cs_entry_src cs_entry_tgt mrel_entry
       mrel_entry i st_src st_tgt
 .
 
-Inductive lsim_func
+Inductive function_lsim
           mrel_init func_src func_tgt: Prop :=
 | lsim_func_intro
     (Hlsim_func_aux: lsim_func_aux mrel_init func_src func_tgt)
     (Hsig: func_src.(fn_sig) = func_tgt.(fn_sig))
 .
 
-End LSIM_FUNC.
+End FUNCTION_LSIM.
 
-Definition lsim prog_src prog_tgt: Prop :=
+Definition program_lsim prog_src prog_tgt: Prop :=
   let ge_src := Genv.globalenv prog_src in
   let ge_tgt := Genv.globalenv prog_tgt in
   forall st_tgt (Hinit_tgt: initial_state prog_tgt st_tgt),
   exists st_src,
     initial_state prog_src st_src /\
   exists mrel_init,
-    Mrel_ops.(sem) mrel_init (state_mem st_src) (state_mem st_tgt) /\
+    mrelT_ops.(sem) mrel_init (state_mem st_src) (state_mem st_tgt) /\
     forall b func_tgt (Hfunc_tgt: Genv.find_funct_ptr ge_tgt b = Some (Internal func_tgt)),
     exists func_src,
       Genv.find_funct_ptr ge_src b = Some (Internal func_src) /\
       True /\ (* TODO: condition on mrel_init and ge_src/tgt. *)
-      lsim_func ge_src ge_tgt mrel_init func_src func_tgt
+      function_lsim ge_src ge_tgt mrel_init func_src func_tgt
 .
 
 End LSIM.
 
-Hint Constructors _lsim_state.
-Hint Resolve lsim_state_mon: paco.
+Hint Constructors _state_lsim.
+Hint Resolve state_lsim_mon: paco.
