common/ProgramSim.v
@@ -5,6 +5,7 @@ Require Import Maps_linker.
 Require Import Integers Floats Values AST Globalenvs.
 Require Import LinkerSpecification LinkerProp Linkeq.
 Require Import Errors.
+Require Import paco.
 
 Set Implicit Arguments.
 
@@ -26,23 +27,33 @@ Variable (transf_EF: forall (ef:EF_src), res EF_tgt).
 Variable (transf_V: forall (v:V_src), res V_tgt).
 Definition V_sim (v_src:V_src) (v_tgt:V_tgt) := transf_V v_src = OK v_tgt.
 
-Parameter F_sim: forall
-                   (defs_src:PTree.t (globdef Fundef_src V_src))
-                   (defs_tgt:PTree.t (globdef Fundef_tgt V_tgt))
-                   (f_src:F_src) (f_tgt:F_tgt), Prop.
+Definition F_simT :=
+  forall
+    (defs_src:list (positive * globdef Fundef_src V_src))
+    (defs_tgt:list (positive * globdef Fundef_tgt V_tgt))
+    (f_src:F_src) (f_tgt:F_tgt), Prop.
 
-(** definition *)
+Section CORE.
+
+Variable (F_sim:F_simT).
+
+Inductive globvar_sim (v_src:globvar V_src) (v_tgt:globvar V_tgt): Prop :=
+| globvar_sim_intro
+    (Hv: transf_globvar transf_V v_src = OK v_tgt)
+.
+
+(** simulation *)
 Inductive globfun_sim
-          (defs_src:PTree.t (globdef Fundef_src V_src))
-          (defs_tgt:PTree.t (globdef Fundef_tgt V_tgt))
+          (defs_src:list (positive * globdef Fundef_src V_src))
+          (defs_tgt:list (positive * globdef Fundef_tgt V_tgt))
           (g_src:Fundef_src) (g_tgt:Fundef_tgt): Prop :=
 | globfun_sim_i
     f_src f_tgt
     (Hsrc: fundef_src_dec g_src = inl f_src)
     (Htgt: fundef_tgt_dec g_tgt = inl f_tgt)
     (Hsim: forall fdefs_src fdefs_tgt
-                  (Hfdefs_src: globdefs_linkeq fundef_src_dec defs_src fdefs_src)
-                  (Hfdefs_tgt: globdefs_linkeq fundef_tgt_dec defs_tgt fdefs_tgt),
+                  (Hfdefs_src: globdef_list_linkeq fundef_src_dec defs_src fdefs_src)
+                  (Hfdefs_tgt: globdef_list_linkeq fundef_tgt_dec defs_tgt fdefs_tgt),
              F_sim fdefs_src fdefs_tgt f_src f_tgt)
 | globfun_sim_e
     ef_src ef_tgt (Hef: transf_EF ef_src = OK ef_tgt)
@@ -51,27 +62,16 @@ Inductive globfun_sim
 .
 
 Inductive globdef_sim
-          (defs_src:PTree.t (globdef Fundef_src V_src))
-          (defs_tgt:PTree.t (globdef Fundef_tgt V_tgt)):
+          (defs_src:list (positive * globdef Fundef_src V_src))
+          (defs_tgt:list (positive * globdef Fundef_tgt V_tgt)):
   forall (g_src:globdef Fundef_src V_src) (g_tgt:globdef Fundef_tgt V_tgt), Prop :=
 | globdef_sim_fun
     f_src f_tgt (Hf: globfun_sim defs_src defs_tgt f_src f_tgt):
     globdef_sim defs_src defs_tgt (Gfun f_src) (Gfun f_tgt)
 | globdef_sim_var
-    v_src v_tgt (Hv: transf_globvar transf_V v_src = OK v_tgt):
+    v_src v_tgt (Hv: globvar_sim v_src v_tgt):
     globdef_sim defs_src defs_tgt (Gvar v_src) (Gvar v_tgt)
 .
-
-Definition globdefs_sim
-           (defs_src:PTree.t (globdef Fundef_src V_src))
-           (defs_tgt:PTree.t (globdef Fundef_tgt V_tgt)):
-  Prop :=
-  forall i,
-    match PTree.get i defs_src, PTree.get i defs_tgt with
-      | Some g1, Some g2 => globdef_sim defs_src defs_tgt g1 g2
-      | None, None => True
-      | _, _ => False
-    end.
 
 Definition globdef_list_sim
            (defs_src:list (positive * globdef Fundef_src V_src))
@@ -80,57 +80,58 @@ Definition globdef_list_sim
   list_forall2
     (fun g_src g_tgt =>
        fst g_src = fst g_tgt /\
-       globdef_sim
-         (PTree.unelements defs_src)
-         (PTree.unelements defs_tgt)
-         (snd g_src) (snd g_tgt))
+       globdef_sim defs_src defs_tgt
+                   (snd g_src) (snd g_tgt))
     defs_src defs_tgt.
 
-Definition program_sim
+Definition program_sim_aux
            (p_src:program Fundef_src V_src)
            (p_tgt:program Fundef_tgt V_tgt): Prop :=
   globdef_list_sim p_src.(prog_defs) p_tgt.(prog_defs) /\
   p_src.(prog_main) = p_tgt.(prog_main).
 
-Lemma globdefs_sim_globdef_list_sim
-      (defs_src: PTree.t (globdef Fundef_src V_src))
-      (defs_tgt: PTree.t (globdef Fundef_tgt V_tgt))
-      (Hsim: globdefs_sim defs_src defs_tgt):
-  globdef_list_sim (PTree.elements defs_src) (PTree.elements defs_tgt).
+End CORE.
+
+(** properties on F_sim and simulation *)
+Lemma globfun_sim_le
+      (F_sim1 F_sim2:F_simT) (HF_sim: F_sim1 <4= F_sim2):
+  (globfun_sim F_sim1) <4= (globfun_sim F_sim2).
 Proof.
-  apply PTree.elements_canonical_order; intros.
-  - exploit Hsim. instantiate (1 := i). rewrite H. intro X.
-    destruct (defs_tgt ! i) eqn:Hi_tgt; [|inv X].
-    eexists. split; eauto.
-    admit. (* TODO: PTree.elements, PTree.unelements *)
-  - exploit Hsim. instantiate (1 := i). rewrite H. intro X.
-    destruct (defs_src ! i) eqn:Hi_src; [|inv X].
-    eexists. split; eauto.
-    admit. (* TODO: PTree.elements, PTree.unelements *)
+  intros. inv PR.
+  - eapply globfun_sim_i; eauto.
+  - eapply globfun_sim_e; eauto.
 Qed.
 
-Lemma globdef_list_sim_globdefs_sim
-      (defs_src: list (positive * globdef Fundef_src V_src))
-      (defs_tgt: list (positive * globdef Fundef_tgt V_tgt))
-      (Hsim: globdef_list_sim defs_src defs_tgt):
-  globdefs_sim (PTree.unelements defs_src) (PTree.unelements defs_tgt).
+Lemma globdef_sim_le
+      (F_sim1 F_sim2:F_simT) (HF_sim: F_sim1 <4= F_sim2):
+  (globdef_sim F_sim1) <4= (globdef_sim F_sim2).
 Proof.
-  unfold globdefs_sim, globdef_list_sim in *.
-  revert Hsim.
-  generalize (PTree.unelements defs_tgt) at 1 3 as defs_tgt'.
-  generalize (PTree.unelements defs_src) at 1 3 as defs_src'.
-  intros defs_src' defs_tgt' Hsim.
-  unfold PTree.unelements. rewrite <- ? fold_left_rev_right.
-  apply list_forall2_rev in Hsim. revert Hsim.
-  generalize (rev defs_src) (rev defs_tgt).
-  clear defs_src defs_tgt.
-  induction l; intros l2 H; inv H; simpl.
-  { intro. rewrite ? PTree.gempty. auto. }
-  destruct H2, a, b1. simpl in *. subst.
-  intro. rewrite ? PTree.gsspec. destruct (peq i p0); subst; auto.
-  apply IHl. auto.
+  intros. inv PR.
+  - eapply globdef_sim_fun; eauto.
+    eapply globfun_sim_le; eauto.
+  - eapply globdef_sim_var; eauto.
 Qed.
 
+Lemma globdef_list_sim_le
+      (F_sim1 F_sim2:F_simT) (HF_sim: F_sim1 <4= F_sim2):
+  (globdef_list_sim F_sim1) <2= (globdef_list_sim F_sim2).
+Proof.
+  intros.
+  eapply list_forall2_imply; eauto. simpl. intros.
+  destruct H1, v1, v2. simpl in *. subst.
+  split; auto. eapply globdef_sim_le; eauto.
+Qed.
+
+Lemma program_sim_aux_le
+      (F_sim1 F_sim2:F_simT) (HF_sim: F_sim1 <4= F_sim2):
+  (program_sim_aux F_sim1) <2= (program_sim_aux F_sim2).
+Proof.
+  intros. destruct PR as [Hdefs Hmain]. split; auto.
+  eapply globdef_list_sim_le; [|eauto]. auto.
+Qed.
+
+(** an instantiation of weak simulation: matching any function definitions *)
+Definition globdef_list_weak_sim := globdef_list_sim (fun _ _ _ _ => True).
 
 (** properties of linking on simulation *)
 Ltac simplify_decs :=
@@ -147,116 +148,29 @@ Ltac simplify_decs :=
         rewrite Hl in Hr; inv Hr
     end.
 
-Lemma link_globdefs_sim
-      (defs1_src defs2_src:PTree.t (globdef Fundef_src V_src))
-      (defs1_tgt defs2_tgt:PTree.t (globdef Fundef_tgt V_tgt))
-      defs_src (Hdefs_src: link_globdefs fundef_src_dec EF_src_dec V_src_dec defs1_src defs2_src = Some defs_src)
-      (H1: globdefs_sim defs1_src defs1_tgt)
-      (H2: globdefs_sim defs2_src defs2_tgt):
-  exists defs_tgt,
-    link_globdefs fundef_tgt_dec EF_tgt_dec V_tgt_dec defs1_tgt defs2_tgt = Some defs_tgt /\
-    globdefs_sim defs_src defs_tgt.
-Proof.
-  generalize (link_globdefs_linkeq_l _ _ _ _ _ Hdefs_src). intro Hle1_src.
-  generalize (link_globdefs_linkeq_r _ _ _ _ _ Hdefs_src). intro Hle2_src.
-  destruct (link_globdefs fundef_tgt_dec EF_tgt_dec V_tgt_dec defs1_tgt defs2_tgt) eqn:Hdefs_tgt.
-  { generalize (link_globdefs_linkeq_l _ _ _ _ _ Hdefs_tgt). intro Hle1_tgt.
-    generalize (link_globdefs_linkeq_r _ _ _ _ _ Hdefs_tgt). intro Hle2_tgt.
-    eexists. split; [eauto|].
-    intro i. rename t into defs_tgt.
-    eapply gtlink_globdefs in Hdefs_src. instantiate (1 := i) in Hdefs_src.
-    eapply gtlink_globdefs in Hdefs_tgt. instantiate (1 := i) in Hdefs_tgt.
-    specialize (H1 i). specialize (H2 i).
-    destruct (defs1_src ! i) eqn:Hi1_src, (defs2_src ! i) eqn:Hi2_src, (defs_src ! i) eqn:Hi_src; subst; try (inv Hdefs_src; fail);
-    destruct (defs1_tgt ! i) eqn:Hi1_tgt, (defs2_tgt ! i) eqn:Hi2_tgt, (defs_tgt ! i) eqn:Hi_tgt; subst; try (inv Hdefs_tgt; fail);
-    try (inv H1; fail); try (inv H2; fail); auto.
-    { destruct Hdefs_src as [[]|[]], Hdefs_tgt as [[]|[]]; subst; auto.
-      { inv H; inv H1; inv H2; inv H3; inv Hv; inv Hv0; try inv Hf; try inv Hf0; simplify_decs.
-        { repeat constructor. eapply globfun_sim_i; eauto.
-          intros. apply Hsim; etransitivity; eauto.
-        }
-        { repeat constructor. eapply globfun_sim_e; eauto. }
-        { constructor. destruct v1, v2. simpl in *. subst.
-          unfold transf_globvar in *. simpl in *.
-          destruct (transf_V gvar_info0); inv H0. simpl in *.
-          inv Hv1. inv Hv2. simpl in *. subst. auto.
-        }
-      }
-      { inv H; inv H1; inv H2; inv H3; inv Hv; inv Hv0; try inv Hf; try inv Hf0; simplify_decs.
-        { repeat constructor. eapply globfun_sim_e; eauto. }
-        { constructor. destruct v1, v2. simpl in *. subst.
-          unfold transf_globvar in *. simpl in *.
-          destruct (transf_V gvar_info0); inv H0. simpl in *.
-          inv Hv1. inv Hv2. simpl in *. subst. auto.
-        }
-      }
-      { admit. (* TODO *) }
-      { admit. (* TODO *) }
-    }
-    { inv H1; constructor; auto.
-      inv Hf; [eapply globfun_sim_i|eapply globfun_sim_e]; eauto.
-      intros. apply Hsim; etransitivity; eauto.
-    }
-    { inv H2; constructor; auto.
-      inv Hf; [eapply globfun_sim_i|eapply globfun_sim_e]; eauto.
-      intros. apply Hsim; etransitivity; eauto.
-    }
-  }
-  { apply gflink_globdefs in Hdefs_tgt.
-    destruct Hdefs_tgt as [i [def1 [def2 [Hdef1 [Hdef2 [H12 H21]]]]]].
-    specialize (H1 i). rewrite Hdef1 in H1.
-    destruct (defs1_src ! i) eqn:Hi1_src; [|inv H1].
-    specialize (H2 i). rewrite Hdef2 in H2.
-    destruct (defs2_src ! i) eqn:Hi2_src; [|inv H2].
-    eapply gtlink_globdefs in Hdefs_src.
-    instantiate (1 := i) in Hdefs_src.
-    rewrite Hi1_src, Hi2_src in Hdefs_src.
-    destruct (defs_src ! i) eqn:Hi_src; [|inv Hdefs_src].
-    destruct Hdefs_src as [[]|[]]; subst.
-    { inv H1; inv H2; inv H; inv Hv; try inv Hv0; try inv Hf; try inv Hf0; simplify_decs.
-      { contradict H12. constructor. eapply globfun_linkable_ei; eauto. }
-      { contradict H12. constructor. eapply globfun_linkable_ee; eauto. }
-      { contradict H12. constructor.
-        destruct v_src, v_src0. inv Hv1. simpl in *. subst.
-        unfold transf_globvar in *. simpl in *.
-        destruct (transf_V gvar_info0); inv H0; inv H1.
-        constructor; auto.
-      }
-    }
-    { inv H1; inv H2; inv H; inv Hv; try inv Hv0; try inv Hf; try inv Hf0; simplify_decs.
-      { contradict H21. constructor. eapply globfun_linkable_ei; eauto. }
-      { contradict H21. constructor. eapply globfun_linkable_ee; eauto. }
-      { contradict H21. constructor.
-        destruct v_src, v_src0. inv Hv1. simpl in *. subst.
-        unfold transf_globvar in *. simpl in *.
-        destruct (transf_V gvar_info); inv H0; inv H1.
-        constructor; auto.
-      }
-    }
-  }
-Qed.
-
 Lemma link_globdef_list_sim
+      (F_sim:F_simT)
       (defs1_src defs2_src:list (positive * globdef Fundef_src V_src))
       (defs1_tgt defs2_tgt:list (positive * globdef Fundef_tgt V_tgt))
       defs_src (Hdefs_src: link_globdef_list fundef_src_dec EF_src_dec V_src_dec defs1_src defs2_src = Some defs_src)
-      (H1: globdef_list_sim defs1_src defs1_tgt)
-      (H2: globdef_list_sim defs2_src defs2_tgt):
+      (H1: globdef_list_sim F_sim defs1_src defs1_tgt)
+      (H2: globdef_list_sim F_sim defs2_src defs2_tgt):
   exists defs_tgt,
     link_globdef_list fundef_tgt_dec EF_tgt_dec V_tgt_dec defs1_tgt defs2_tgt = Some defs_tgt /\
-    globdef_list_sim defs_src defs_tgt.
+    globdef_list_sim F_sim defs_src defs_tgt.
 Proof.
-  apply globdef_list_sim_globdefs_sim in H1.
-  apply globdef_list_sim_globdefs_sim in H2.
-  unfold link_globdef_list in Hdefs_src.
-  match goal with
-    | [H: context[link_globdefs ?fundef_dec ?EF_dec ?V_dec ?defs1 ?defs2] |- _] =>
-      destruct (link_globdefs fundef_dec EF_dec V_dec defs1 defs2) as [defs|] eqn:Hdefs; inv H
-  end.
-  exploit link_globdefs_sim; eauto. intros [defs_tgt [Hdefs_tgt Hsim]].
-  unfold link_globdef_list. rewrite Hdefs_tgt. eexists. split; eauto.
-  apply globdefs_sim_globdef_list_sim. auto.
+  admit.
 Qed.
+
+Section DEF.
+
+Variable (F_sim:F_simT).
+
+Definition program_sim :=
+  program_sim_aux
+    (fun defs_src defs_tgt f_src f_tgt =>
+       forall (Hdefs: globdef_list_weak_sim defs_src defs_tgt),
+       F_sim defs_src defs_tgt f_src f_tgt).
 
 Lemma link_program_sim
       (p1_src p2_src:program Fundef_src V_src)
@@ -283,16 +197,20 @@ Proof.
   split; auto.
 Qed.
 
+End DEF.
+
 Section INITIALIZE.
 
+Variable (F_sim:F_simT).
 Variable (p_src: program Fundef_src V_src).
 Variable (p_tgt: program Fundef_tgt V_tgt).
-Variable (Hp: program_sim p_src p_tgt).
+Variable (Hp: program_sim_aux F_sim p_src p_tgt).
 
 Definition match_fundef :=
   globfun_sim
-    (PTree.unelements p_src.(prog_defs))
-    (PTree.unelements p_tgt.(prog_defs)).
+    F_sim
+    p_src.(prog_defs)
+    p_tgt.(prog_defs).
 
 Lemma program_sim_match_program:
   match_program match_fundef V_sim nil p_src.(prog_main) p_src p_tgt.
@@ -305,8 +223,8 @@ Proof.
   destruct v1 as [var1 g1], v2 as [var2 g2]. simpl in *. subst.
   inv H2.
   - constructor. auto.
-  - destruct v_src. unfold transf_globvar in Hv. simpl in Hv.
-    destruct (transf_V gvar_info) eqn:Hinfo; inv Hv. simpl in *.
+  - inv Hv. destruct v_src. unfold transf_globvar in Hv0. simpl in Hv0.
+    destruct (transf_V gvar_info) eqn:Hinfo; inv Hv0. simpl in *.
     constructor. auto.
 Qed.
 
