backend/MemoryRelation.v
@@ -6,57 +6,57 @@ Set Implicit Arguments.
 
 (* signature *)
 
-Record MREL_ops (t:Type): Type := mkMREL_ops {
+Record mrelT_opsT (t:Type): Type := mkmrelT_opsT {
   sem :> t -> forall (m1 m2:mem), Prop;
   sem_value :> t -> forall (v1 v2:val), Prop;
   le: t -> t -> Prop;
   le_public: t -> t -> Prop
 }.
 
-Record MREL_props (t:Type) (ops:MREL_ops t): Prop := mkMREL_props {
+Record mrelT_props (t:Type) (ops:mrelT_opsT t): Prop := mkmrelT_props {
   le_public_le:
     forall mrel1 mrel2 (Hle_public: ops.(le_public) mrel1 mrel2),
       ops.(le) mrel1 mrel2
 }.
 
-Record MREL: Type := mkMREL {
+Record mrelT: Type := mkmrelT {
   t :> Type;
-  ops: MREL_ops t;
-  props: MREL_props ops
+  ops: mrelT_opsT t;
+  props: mrelT_props ops
 }.
 
 
 (* equals *)
 
-Definition MREL_ops_equals: MREL_ops unit :=
-  mkMREL_ops
+Definition mrelT_ops_equals: mrelT_opsT unit :=
+  mkmrelT_opsT
     (fun _ m1 m2 => m1 = m2)
     (fun _ v1 v2 => Val.lessdef v1 v2)
     (fun _ _ => True)
     (fun _ _ => True).
 
-Program Definition MREL_props_equals: MREL_props MREL_ops_equals := mkMREL_props _ _.
+Program Definition mrelT_props_equals: mrelT_props mrelT_ops_equals := mkmrelT_props _ _.
 
 
 (* extends *)
 
-Definition MREL_ops_extends: MREL_ops unit :=
-  mkMREL_ops
+Definition mrelT_ops_extends: mrelT_opsT unit :=
+  mkmrelT_opsT
     (fun _ m1 m2 => Mem.extends m1 m2)
     (fun _ v1 v2 => Val.lessdef v1 v2)
     (fun _ _ => True)
     (fun _ _ => True).
 
-Program Definition MREL_props_extends: MREL_props MREL_ops_extends := mkMREL_props _ _.
+Program Definition mrelT_props_extends: mrelT_props mrelT_ops_extends := mkmrelT_props _ _.
 
 
 (* inject *)
 
-Definition MREL_ops_inject: MREL_ops meminj :=
-  mkMREL_ops
+Definition mrelT_ops_inject: mrelT_opsT meminj :=
+  mkmrelT_opsT
     Mem.inject
     val_inject
     inject_incr
     inject_incr.
 
-Program Definition MREL_props_inject: MREL_props MREL_ops_inject := mkMREL_props _ _.
+Program Definition mrelT_props_inject: mrelT_props mrelT_ops_inject := mkmrelT_props _ _.
